Isabelle/INTO-CPS/INTO_SysML_3WTs_toCSP.thy
@@ -1,10 +1,11 @@
 
-(*  Title:      Converts the water tanks models into CSPm files that can be run in FDR3
-    Author:     Nuno Amálio
+(*  Theory:      'INTO_SysML_3WTs_toCSP'
+    Description: Generates CSPm files for the 3 water tanks models that can be run in FDR3
+    Author:      Nuno Amálio
 *)
 
 theory INTO_SysML_3WTs_toCSP
-imports INTO_SysML_3WTs INTO_SysML_3WTs_loop "CSP/CSP_print" PDG_To_CSP
+imports INTO_SysML_3WTs INTO_SysML_3WTs_loop CSP_print PDG_To_CSP
   
 begin
 
@@ -15,11 +16,11 @@ where
 
 export_code toCSP expid csp str_int INTO_SysML_toPDG
   MdlTy_3WTs MdlTy_3WTs_loop mdlL mtyL output_dir
-  in SML module_name CSP file "CSP/csp.sml"
+  in SML module_name CSP file "csp.sml"
 
-ML_file "CSP/csp.sml"
+ML_file "csp.sml"
 
-ML_file "CSP/wr-csp.sml"
+ML_file "wr-csp.sml"
 
 ML {*
 (*val dir1 = OS.FileSys.getDir();*)
